ulib/FStar.Monotonic.HyperHeap.fst
@@ -20,78 +20,52 @@ open FStar.Monotonic.Heap
 module Map = FStar.Map
 open FStar.Ghost
 
-abstract type hh_rid = erased (list (int * int))
+abstract type rid = erased (list (int * int))
 
-let reveal (r:hh_rid) : GTot (list (int * int)) = reveal r
+let reveal (r:rid) : GTot (list (int * int)) = reveal r
 
-abstract let hh_color (x:hh_rid): GTot int =
+abstract let color (x:rid): GTot int =
   match reveal x with
   | [] -> 0
   | (c, _)::_ -> c
 
-type t = Map.t hh_rid heap
+type t = Map.t rid heap
 
 let has_eq_rid (u:unit) :
   Lemma (requires True)
-        (ensures hasEq hh_rid)
+        (ensures hasEq rid)
   = ()
 
-assume HasEq_rid: hasEq hh_rid //TODO: we just proved this above, but we need to expose it as an argument-free SMT lemma, which isn't supported yet
+assume HasEq_rid: hasEq rid //TODO: we just proved this above, but we need to expose it as an argument-free SMT lemma, which isn't supported yet
 
 (* AR: see issue#1262 *)
-abstract let hh_root :hh_rid = let x:hh_rid = hide [] in x
+abstract let root :rid = let x:rid = hide [] in x
 
 //is this SMTPat bad ?
-val lemma_root_has_color_zero: r:hh_rid{r == hh_root}
-                               -> Lemma (requires True) (ensures (hh_color r = 0))
-                                 [SMTPat (hh_color r)]
+val lemma_root_has_color_zero: r:rid{r == root}
+                               -> Lemma (requires True) (ensures (color r = 0))
+                                 [SMTPat (color r)]
 let lemma_root_has_color_zero r = ()
 
 //expose this so that no-one should assume otheriwse
-let root_has_color_zero (u:unit) :Lemma (hh_color hh_root = 0) = ()
+let root_has_color_zero (u:unit) :Lemma (color root = 0) = ()
 
-abstract type mrref (id:hh_rid) (a:Type) (rel:preorder a) = mref a rel
-
-(* let has_eq_rref (id:hh_rid) (a:Type) : *)
-(*   Lemma (requires True) *)
-(*         (ensures hasEq (rref id a)) *)
-(*      [SMTPat (hasEq (rref id a))] *)
-(*   = ()        *)
-
-abstract val as_ref : #a:Type -> #id:hh_rid -> #rel:preorder a -> r:mrref id a rel -> Tot (mref a rel)
-let as_ref #a #id #rel r = r
-
-val addr_of: #a:Type -> #id:hh_rid -> #rel:preorder a -> r:mrref id a rel -> GTot nat
-let addr_of #a #id #rel r = addr_of (as_ref r)
-
-let is_mm (#a:Type) (#id:hh_rid) (#rel:preorder a) (r:mrref id a rel) :GTot bool
-  = is_mm (as_ref r)
-
-abstract val ref_as_rref : #a:Type -> #rel:preorder a -> i:hh_rid -> r:mref a rel -> GTot (mrref i a rel)
-let ref_as_rref #a #rel i r = r
-
-val lemma_as_ref_inj: #a:Type -> #i:hh_rid -> #rel:preorder a -> r:mrref i a rel
-    -> Lemma (requires (True))
-             (ensures ((ref_as_rref i (as_ref r) == r)))
-       [SMTPat (as_ref r)]
-let lemma_as_ref_inj #a #i #rel r = ()
-
-private let rid_tail (r:hh_rid{Cons? (reveal r)}) :hh_rid =
+private let rid_tail (r:rid{Cons? (reveal r)}) :rid =
   elift1_p Cons?.tl r
 
-private let rid_length (r:hh_rid) :GTot nat = List.Tot.length (reveal r)
+private let rid_length (r:rid) :GTot nat = List.Tot.length (reveal r)
 
-abstract val includes : r1:hh_rid -> r2:hh_rid -> GTot bool (decreases (reveal r2))
+abstract val includes : r1:rid -> r2:rid -> GTot bool (decreases (reveal r2))
 let rec includes r1 r2 =
   if r1=r2 then true
   else if rid_length r2 > rid_length r1
   then includes r1 (rid_tail r2)
   else false
 
-let disjoint (i:hh_rid) (j:hh_rid) : GTot bool =
+let disjoint (i:rid) (j:rid) : GTot bool =
   not (includes i j) && not (includes j i)
 
-private val lemma_aux: k:hh_rid -> i:hh_rid
+private val lemma_aux: k:rid -> i:rid
       -> Lemma  (requires
                     rid_length k > 0
                     /\ rid_length k <= rid_length i
@@ -101,7 +75,7 @@ private val lemma_aux: k:hh_rid -> i:hh_rid
                  (decreases (rid_length i))
 let rec lemma_aux k i = lemma_aux k (rid_tail i)
 
-abstract val lemma_disjoint_includes: i:hh_rid -> j:hh_rid -> k:hh_rid ->
+abstract val lemma_disjoint_includes: i:rid -> j:rid -> k:rid ->
   Lemma (requires (disjoint i j /\ includes j k))
         (ensures (disjoint i k))
         (decreases (List.Tot.length (reveal k)))
@@ -117,98 +91,89 @@ let rec lemma_disjoint_includes i j k =
               then lemma_aux k i
               else ()))
 
-abstract val extends: hh_rid -> hh_rid -> GTot bool
+abstract val extends: rid -> rid -> GTot bool
 let extends r0 r1 = Cons? (reveal r0) && rid_tail r0 = r1
 
-abstract val parent: r:hh_rid{r<>hh_root} -> Tot hh_rid
+abstract val parent: r:rid{r<>root} -> Tot rid
 let parent r = rid_tail r
 
-abstract val lemma_includes_refl: i:hh_rid
+abstract val lemma_includes_refl: i:rid
                       -> Lemma (requires (True))
                                (ensures (includes i i))
                                [SMTPat (includes i i)]
 let lemma_includes_refl i = ()
 
-abstract val lemma_extends_includes: i:hh_rid -> j:hh_rid ->
+abstract val lemma_extends_includes: i:rid -> j:rid ->
   Lemma (requires (extends j i))
         (ensures (includes i j /\ not(includes j i)))
         [SMTPat (extends j i)]
 let lemma_extends_includes i j = ()
 
-let lemma_includes_anti_symmetric (i:hh_rid) (j:hh_rid) :
+let lemma_includes_anti_symmetric (i:rid) (j:rid) :
   Lemma (requires (includes i j /\ i <> j))
         (ensures (not (includes j i)))
         [SMTPat (includes i j)]
   = ()
 
-abstract val lemma_extends_disjoint: i:hh_rid -> j:hh_rid -> k:hh_rid ->
+abstract val lemma_extends_disjoint: i:rid -> j:rid -> k:rid ->
     Lemma (requires (extends j i /\ extends k i /\ j<>k))
           (ensures (disjoint j k))
 let lemma_extends_disjoint i j k = ()
 
-abstract val lemma_extends_parent: i:hh_rid{i<>hh_root} ->
+abstract val lemma_extends_parent: i:rid{i<>root} ->
   Lemma (requires True)
         (ensures (extends i (parent i)))
         [SMTPat (parent i)]
 let lemma_extends_parent i = ()
 
-abstract val lemma_extends_not_root: i:hh_rid -> j:hh_rid{extends j i} ->
+abstract val lemma_extends_not_root: i:rid -> j:rid{extends j i} ->
   Lemma (requires True)
-        (ensures (j<>hh_root))
+        (ensures (j<>root))
         [SMTPat (extends j i)]
 let lemma_extends_not_root i j = ()
 
-abstract val lemma_extends_only_parent: i:hh_rid -> j:hh_rid{extends j i} ->
+abstract val lemma_extends_only_parent: i:rid -> j:rid{extends j i} ->
   Lemma (requires True)
         (ensures (i = parent j))
         [SMTPat (extends j i)]
 let lemma_extends_only_parent i j = ()
 
 private let test0 = assert (includes (hide [(0, 1) ; (1, 0)]) (hide [(2, 2); (0, 1); (1, 0)]))
-private let test1 (r1:hh_rid) (r2:hh_rid{includes r1 r2}) = assert (includes r1 (hide ((0,0)::(reveal r2))))
+private let test1 (r1:rid) (r2:rid{includes r1 r2}) = assert (includes r1 (hide ((0,0)::(reveal r2))))
 
 
-let sel (#a:Type) (#rel:preorder a) (#i:hh_rid) (m:t) (r:mrref i a rel) : GTot a
-  = sel (Map.sel m i) (as_ref r)
-unfold let op_String_Access (#a:Type) (#rel:preorder a) (#i:hh_rid) (m:t) (r:mrref i a rel) = sel m r
+assume val mod_set : Set.set rid -> Tot (Set.set rid)
+assume Mod_set_def: forall (x:rid) (s:Set.set rid). {:pattern Set.mem x (mod_set s)}
+                    Set.mem x (mod_set s) <==> (exists (y:rid). Set.mem y s /\ includes y x)
 
-let upd (#a:Type) (#rel:preorder a) (#i:hh_rid) (m:t) (r:mrref i a rel) (v:a) :GTot t
-  = Map.upd m i (upd (Map.sel m i) (as_ref r) v)
-unfold let op_String_Assignment (#a:Type) (#rel:preorder a) (#i:hh_rid) (m:t) (r:mrref i a rel) v = upd m r v
-
-
-assume val mod_set : Set.set hh_rid -> Tot (Set.set hh_rid)
-assume Mod_set_def: forall (x:hh_rid) (s:Set.set hh_rid). {:pattern Set.mem x (mod_set s)}
-                    Set.mem x (mod_set s) <==> (exists (y:hh_rid). Set.mem y s /\ includes y x)
-
-let modifies (s:Set.set hh_rid) (m0:t) (m1:t) =
+let modifies (s:Set.set rid) (m0:t) (m1:t) =
   Map.equal m1 (Map.concat m1 (Map.restrict (Set.complement (mod_set s)) m0))
   /\ Set.subset (Map.domain m0) (Map.domain m1)
 
-let modifies_just (s:Set.set hh_rid) (m0:t) (m1:t) =
+let modifies_just (s:Set.set rid) (m0:t) (m1:t) =
   Map.equal m1 (Map.concat m1 (Map.restrict (Set.complement s) m0))
   /\ Set.subset (Map.domain m0) (Map.domain m1)
 
-let modifies_one (r:hh_rid) (m0:t) (m1:t) =
+let modifies_one (r:rid) (m0:t) (m1:t) =
   modifies_just (Set.singleton r) m0 m1
 
-let equal_on (s:Set.set hh_rid) (m0:t) (m1:t) =
- (forall (r:hh_rid). {:pattern (Map.contains m0 r)} (Set.mem r (mod_set s) /\ Map.contains m0 r) ==> Map.contains m1 r)
+let equal_on (s:Set.set rid) (m0:t) (m1:t) =
+ (forall (r:rid). {:pattern (Map.contains m0 r)} (Set.mem r (mod_set s) /\ Map.contains m0 r) ==> Map.contains m1 r)
  /\ Map.equal m1 (Map.concat m1 (Map.restrict (mod_set s) m0))
 
 abstract val lemma_modifies_just_trans: m1:t -> m2:t -> m3:t
-                       -> s1:Set.set hh_rid -> s2:Set.set hh_rid
+                       -> s1:Set.set rid -> s2:Set.set rid
                        -> Lemma (requires (modifies_just s1 m1 m2 /\ modifies_just s2 m2 m3))
                                (ensures (modifies_just (Set.union s1 s2) m1 m3))
 let lemma_modifies_just_trans m1 m2 m3 s1 s2 = ()
 
 abstract val lemma_modifies_trans: m1:t -> m2:t -> m3:t
-                       -> s1:Set.set hh_rid -> s2:Set.set hh_rid
+                       -> s1:Set.set rid -> s2:Set.set rid
                        -> Lemma (requires (modifies s1 m1 m2 /\ modifies s2 m2 m3))
                                (ensures (modifies (Set.union s1 s2) m1 m3))
 let lemma_modifies_trans m1 m2 m3 s1 s2 = ()
 
-abstract val lemma_includes_trans: i:hh_rid -> j:hh_rid -> k:hh_rid
+abstract val lemma_includes_trans: i:rid -> j:rid -> k:rid
                         -> Lemma (requires (includes i j /\ includes j k))
                                 (ensures (includes i k))
 				(decreases (reveal k))
@@ -219,24 +184,24 @@ let rec lemma_includes_trans i j k =
   else match reveal k with
         | hd::tl -> lemma_includes_trans i j (hide tl)
 
-abstract val lemma_modset: i:hh_rid -> j:hh_rid
+abstract val lemma_modset: i:rid -> j:rid
                   -> Lemma (requires (includes j i))
                            (ensures (Set.subset (mod_set (Set.singleton i)) (mod_set (Set.singleton j))))
 let lemma_modset i j = ()
 
 abstract val lemma_modifies_includes: m1:t -> m2:t
-                       -> i:hh_rid -> j:hh_rid
+                       -> i:rid -> j:rid
                        -> Lemma (requires (modifies (Set.singleton i) m1 m2 /\ includes j i))
                                 (ensures (modifies (Set.singleton j) m1 m2))
 let lemma_modifies_includes m1 m2 i j = ()
 
 abstract val lemma_modifies_includes2: m1:t -> m2:t
-                       -> s1:Set.set hh_rid -> s2:Set.set hh_rid
+                       -> s1:Set.set rid -> s2:Set.set rid
                        -> Lemma (requires (modifies s1 m1 m2 /\ (forall x.  Set.mem x s1 ==> (exists y. Set.mem y s2 /\ includes y x))))
                                 (ensures (modifies s2 m1 m2))
 let lemma_modifies_includes2 m1 m2 s1 s2 = ()
 
-abstract val lemma_disjoint_parents: pr:hh_rid -> r:hh_rid -> ps:hh_rid -> s:hh_rid -> Lemma
+abstract val lemma_disjoint_parents: pr:rid -> r:rid -> ps:rid -> s:rid -> Lemma
   (requires (r `extends` pr /\ s `extends` ps /\ disjoint pr ps))
   (ensures (disjoint r s))
   [SMTPat (extends r pr); SMTPat (extends s ps); SMTPat (disjoint pr ps)]
@@ -244,42 +209,32 @@ let lemma_disjoint_parents pr r ps s =
     assert (pr `includes` r);
     assert (ps `includes` s)
 
-let unused_in (#a:Type) (#rel:preorder a) (#i:hh_rid) (r:mrref i a rel) (m:t) :GTot bool =
-  not (Map.contains m i) ||
-  FStar.StrongExcludedMiddle.strong_excluded_middle (Heap.unused_in (as_ref r) (Map.sel m i))
-
-let contains_ref_in_its_region (#a:Type) (#rel:preorder a) (#i:hh_rid) (r:mrref i a rel) (m:t) : GTot bool =
-  FStar.StrongExcludedMiddle.strong_excluded_middle (Heap.contains (Map.sel m i) (as_ref r))
-
-let modifies_rref (r:hh_rid) (s:Set.set nat) h0 h1 =
-  Heap.modifies s (Map.sel h0 r) (Map.sel h1 r)
-
-abstract val lemma_include_cons: i:hh_rid -> j:hh_rid -> Lemma
+abstract val lemma_include_cons: i:rid -> j:rid -> Lemma
   (requires (i<>j /\ includes i j))
-  (ensures (j<>hh_root))
+  (ensures (j<>root))
 let lemma_include_cons i j = ()
 
 let map_invariant (m:t) =
   forall r. Map.contains m r ==>
       (forall s. includes s r ==> Map.contains m s)
 
-let disjoint_regions (s1:Set.set hh_rid) (s2:Set.set hh_rid) =
+let disjoint_regions (s1:Set.set rid) (s2:Set.set rid) =
      forall x y. {:pattern (Set.mem x s1); (Set.mem y s2)} (Set.mem x s1 /\ Set.mem y s2) ==> disjoint x y
 
-let extends_parent (tip:hh_rid{tip<>hh_root}) (r:hh_rid)
+let extends_parent (tip:rid{tip<>root}) (r:rid)
   : Lemma (ensures (extends r (parent tip) /\ r<>tip ==> disjoint r tip \/ extends r tip))
           [SMTPat (extends r (parent tip))]
   = ()
 
-let includes_child (tip:hh_rid{tip<>hh_root}) (r:hh_rid)
+let includes_child (tip:rid{tip<>root}) (r:rid)
   : Lemma (ensures (includes r tip ==> r=tip \/ includes r (parent tip)))
           [SMTPat (includes r (parent tip))]
   = ()
 
-let root_is_root (s:hh_rid)
-  : Lemma (requires (includes s hh_root))
-          (ensures (s = hh_root))
-          [SMTPat (includes s hh_root)]
+let root_is_root (s:rid)
+  : Lemma (requires (includes s root))
+          (ensures (s = root))
+          [SMTPat (includes s root)]
   = ()
 
 (*
@@ -290,236 +245,236 @@ let root_is_root (s:hh_rid)
 
 (* Definition and ghost decidable equality *)
 
-abstract let aref (i: hh_rid) : Type0 = Heap.aref
+// abstract let aref (i: rid) : Type0 = Heap.aref
 
-abstract let as_heap_aref (#i:hh_rid) (r:aref i) :Heap.aref = r
+// abstract let as_heap_aref (#i:rid) (r:aref i) :Heap.aref = r
 
-abstract let heap_aref_as_aref (i:hh_rid) (r:Heap.aref) :aref i = r
+// abstract let heap_aref_as_aref (i:rid) (r:Heap.aref) :aref i = r
 
-let lemma_as_aref_injective (#i:hh_rid) (r:aref i)
-  :Lemma (requires True)
-         (ensures  (heap_aref_as_aref i (as_heap_aref r) == r))
-	 [SMTPat (as_heap_aref r)]
-  = ()
+// let lemma_as_aref_injective (#i:rid) (r:aref i)
+//   :Lemma (requires True)
+//          (ensures  (heap_aref_as_aref i (as_heap_aref r) == r))
+// 	 [SMTPat (as_heap_aref r)]
+//   = ()
 
-abstract let dummy_aref (i: hh_rid) : aref i = Heap.dummy_aref
+// abstract let dummy_aref (i: rid) : aref i = Heap.dummy_aref
 
-let aref_equal
-  (#i: hh_rid)
-  (a1 a2: aref i)
-: Ghost bool
-  (requires True)
-  (ensures (fun b -> b == true <==> a1 == a2))
-= Heap.aref_equal (as_heap_aref a1) (as_heap_aref a2)
+// let aref_equal
+//   (#i: rid)
+//   (a1 a2: aref i)
+// : Ghost bool
+//   (requires True)
+//   (ensures (fun b -> b == true <==> a1 == a2))
+// = Heap.aref_equal (as_heap_aref a1) (as_heap_aref a2)
 
-(* Introduction rule *)
+// (* Introduction rule *)
 
-let aref_of
-  (#i: hh_rid)
-  (#a: Type)
-  (#rel: preorder a)
-  (r: mrref i a rel)
-: Tot (aref i)
-= Heap.aref_of (as_ref r)
+// let aref_of
+//   (#i: rid)
+//   (#a: Type)
+//   (#rel: preorder a)
+//   (r: mrref i a rel)
+// : Tot (aref i)
+// = Heap.aref_of (as_ref r)
 
-(* Operators lifted from rref *)
+// (* Operators lifted from rref *)
 
-let addr_of_aref
-  (#id:hh_rid)
-  (r:aref id)
-: GTot nat
-= Heap.addr_of_aref (as_heap_aref r)
+// let addr_of_aref
+//   (#id:rid)
+//   (r:aref id)
+// : GTot nat
+// = Heap.addr_of_aref (as_heap_aref r)
 
-let addr_of_aref_of
-  (#id:hh_rid)
-  (#a: Type)
-  (#rel: preorder a)
-  (r: mrref id a rel)
-: Lemma
-  (addr_of r == addr_of_aref (aref_of r))
-  [SMTPat (addr_of_aref (aref_of r))]
-= Heap.addr_of_aref_of (as_ref r)
-
-let aref_is_mm
-  (#id: hh_rid)
-  (r: aref id)
-: GTot bool
-= Heap.aref_is_mm (as_heap_aref r)
-
-let is_mm_aref_of
-  (#id: hh_rid)
-  (#a: Type)
-  (#rel: preorder a)
-  (r: mrref id a rel)
-: Lemma
-  (is_mm r == aref_is_mm (aref_of r))
-  [SMTPat (aref_is_mm (aref_of r))]
-= Heap.is_mm_aref_of (as_ref r)
-
-let aref_unused_in
-  (#i: hh_rid)
-  (r: aref i)
-  (m: t)
-: GTot Type0
-= not (Map.contains m i) \/
-  Heap.aref_unused_in (as_heap_aref r) (Map.sel m i)
-
-let unused_in_aref_of
-  (#i: hh_rid)
-  (#a: Type)
-  (#rel: preorder a)
-  (r: mrref i a rel)
-  (m: t)
-: Lemma
-  (aref_unused_in (aref_of r) m <==> unused_in r m)
-  [SMTPat (aref_unused_in (aref_of r) m)]
-= Heap.unused_in_aref_of (as_ref r) (Map.sel m i)
-
-// abstract
-// val contains_ref_aref_unused_in: #i: hh_rid -> #a:Type -> #rel: preorder a -> h:t -> x:mrref i a rel -> y:aref i -> Lemma
-//   (requires (contains_ref x h /\ aref_unused_in y h))
-//   (ensures  (addr_of x <> addr_of_aref y))
-// let contains_ref_aref_unused_in #i #a #rel h x y = Heap.contains_aref_unused_in (Map.sel h i) x y
-
-(* Elimination rule *)
-
-let aref_live_at (m: t) (#i: hh_rid) (a: aref i) (v: Type) (rel: preorder v) : GTot Type0 =
-  Map.contains m i /\
-  Heap.aref_live_at (Map.sel m i) (as_heap_aref a) v rel
-
-let grref_of
-  (#i: hh_rid)
-  (a: aref i)
-  (v: Type0)
-  (rel: preorder v)
-: Ghost (mrref i v rel)
-  (requires (exists m . aref_live_at m a v rel))
-  (ensures (fun x -> True))
-= Heap.gref_of (as_heap_aref a) v rel
-
-let rref_of
-  (m: t)
-  (#i: hh_rid)
-  (a: aref i)
-  (v: Type)
-  (rel: preorder v)
-: Pure (mrref i v rel)
-  (requires (aref_live_at m a v rel))
-  (ensures (fun x -> aref_live_at m a v rel /\ addr_of x == addr_of_aref a /\ is_mm x == aref_is_mm a))
-= Heap.ref_of (Map.sel m i) (as_heap_aref a) v rel
-
-// abstract
-// let aref_live_at_aref_of
-//   (m: t)
-//   (#i: hh_rid)
-//   (#v: Type0)
-//   (#rel: preorder v)
-//   (r: mrref i v rel)
+// let addr_of_aref_of
+//   (#id:rid)
+//   (#a: Type)
+//   (#rel: preorder a)
+//   (r: mrref id a rel)
 // : Lemma
-//   (ensures (aref_live_at m (aref_of r) v rel <==> contains_ref r m))
-//   [SMTPat (aref_live_at m (aref_of r) v rel)]
-// = ()
+//   (addr_of r == addr_of_aref (aref_of r))
+//   [SMTPat (addr_of_aref (aref_of r))]
+// = Heap.addr_of_aref_of (as_ref r)
 
-// abstract
-// let contains_ref_grref_of
+// let aref_is_mm
+//   (#id: rid)
+//   (r: aref id)
+// : GTot bool
+// = Heap.aref_is_mm (as_heap_aref r)
+
+// let is_mm_aref_of
+//   (#id: rid)
+//   (#a: Type)
+//   (#rel: preorder a)
+//   (r: mrref id a rel)
+// : Lemma
+//   (is_mm r == aref_is_mm (aref_of r))
+//   [SMTPat (aref_is_mm (aref_of r))]
+// = Heap.is_mm_aref_of (as_ref r)
+
+// let aref_unused_in
+//   (#i: rid)
+//   (r: aref i)
 //   (m: t)
-//   (#i: hh_rid)
+// : GTot Type0
+// = not (Map.contains m i) \/
+//   Heap.aref_unused_in (as_heap_aref r) (Map.sel m i)
+
+// let unused_in_aref_of
+//   (#i: rid)
+//   (#a: Type)
+//   (#rel: preorder a)
+//   (r: mrref i a rel)
+//   (m: t)
+// : Lemma
+//   (aref_unused_in (aref_of r) m <==> unused_in r m)
+//   [SMTPat (aref_unused_in (aref_of r) m)]
+// = Heap.unused_in_aref_of (as_ref r) (Map.sel m i)
+
+// // abstract
+// // val contains_ref_aref_unused_in: #i: rid -> #a:Type -> #rel: preorder a -> h:t -> x:mrref i a rel -> y:aref i -> Lemma
+// //   (requires (contains_ref x h /\ aref_unused_in y h))
+// //   (ensures  (addr_of x <> addr_of_aref y))
+// // let contains_ref_aref_unused_in #i #a #rel h x y = Heap.contains_aref_unused_in (Map.sel h i) x y
+
+// (* Elimination rule *)
+
+// let aref_live_at (m: t) (#i: rid) (a: aref i) (v: Type) (rel: preorder v) : GTot Type0 =
+//   Map.contains m i /\
+//   Heap.aref_live_at (Map.sel m i) (as_heap_aref a) v rel
+
+// let grref_of
+//   (#i: rid)
+//   (a: aref i)
+//   (v: Type0)
+//   (rel: preorder v)
+// : Ghost (mrref i v rel)
+//   (requires (exists m . aref_live_at m a v rel))
+//   (ensures (fun x -> True))
+// = Heap.gref_of (as_heap_aref a) v rel
+
+// let rref_of
+//   (m: t)
+//   (#i: rid)
+//   (a: aref i)
+//   (v: Type)
+//   (rel: preorder v)
+// : Pure (mrref i v rel)
+//   (requires (aref_live_at m a v rel))
+//   (ensures (fun x -> aref_live_at m a v rel /\ addr_of x == addr_of_aref a /\ is_mm x == aref_is_mm a))
+// = Heap.ref_of (Map.sel m i) (as_heap_aref a) v rel
+
+// // abstract
+// // let aref_live_at_aref_of
+// //   (m: t)
+// //   (#i: rid)
+// //   (#v: Type0)
+// //   (#rel: preorder v)
+// //   (r: mrref i v rel)
+// // : Lemma
+// //   (ensures (aref_live_at m (aref_of r) v rel <==> contains_ref r m))
+// //   [SMTPat (aref_live_at m (aref_of r) v rel)]
+// // = ()
+
+// // abstract
+// // let contains_ref_grref_of
+// //   (m: t)
+// //   (#i: rid)
+// //   (a: aref i)
+// //   (v: Type0)
+// //   (rel: preorder v)
+// // : Lemma
+// //   (requires (exists h' . aref_live_at h' a v rel))
+// //   (ensures ((exists h' . aref_live_at h' a v rel) /\ (contains_ref (grref_of a v rel) m <==> aref_live_at m a v rel)))
+// //   [SMTPatOr [
+// //     [SMTPat (contains_ref (grref_of a v rel) m)];
+// //     [SMTPat (aref_live_at m a v rel)];
+// //   ]]
+// // = ()
+
+// let aref_of_grref_of
+//   (#i: rid)
 //   (a: aref i)
 //   (v: Type0)
 //   (rel: preorder v)
 // : Lemma
-//   (requires (exists h' . aref_live_at h' a v rel))
-//   (ensures ((exists h' . aref_live_at h' a v rel) /\ (contains_ref (grref_of a v rel) m <==> aref_live_at m a v rel)))
-//   [SMTPatOr [
-//     [SMTPat (contains_ref (grref_of a v rel) m)];
-//     [SMTPat (aref_live_at m a v rel)];
-//   ]]
+//   (requires (exists h . aref_live_at h a v rel))
+//   (ensures ((exists h. aref_live_at h a v rel) /\ aref_of (grref_of a v rel) == a))
+//   [SMTPat (aref_of (grref_of a v rel))]
 // = ()
 
-let aref_of_grref_of
-  (#i: hh_rid)
-  (a: aref i)
-  (v: Type0)
-  (rel: preorder v)
-: Lemma
-  (requires (exists h . aref_live_at h a v rel))
-  (ensures ((exists h. aref_live_at h a v rel) /\ aref_of (grref_of a v rel) == a))
-  [SMTPat (aref_of (grref_of a v rel))]
-= ()
+// (* Operators lowered to rref *)
 
-(* Operators lowered to rref *)
+// let addr_of_grref_of
+//   (#i: rid)
+//   (a: aref i)
+//   (t: Type0)
+//   (rel: preorder t)
+// : Lemma
+//   (requires (exists h . aref_live_at h a t rel))
+//   (ensures ((exists h . aref_live_at h a t rel) /\ addr_of (grref_of a t rel) == addr_of_aref a))
+//   [SMTPat (addr_of (grref_of a t rel))]
+// = ()
 
-let addr_of_grref_of
-  (#i: hh_rid)
-  (a: aref i)
-  (t: Type0)
-  (rel: preorder t)
-: Lemma
-  (requires (exists h . aref_live_at h a t rel))
-  (ensures ((exists h . aref_live_at h a t rel) /\ addr_of (grref_of a t rel) == addr_of_aref a))
-  [SMTPat (addr_of (grref_of a t rel))]
-= ()
+// let is_mm_grref_of
+//   (#i: rid)
+//   (a: aref i)
+//   (t: Type0)
+//   (rel: preorder t)
+// : Lemma
+//   (requires (exists h . aref_live_at h a t rel))
+//   (ensures ((exists h . aref_live_at h a t rel) /\ is_mm (grref_of a t rel) == aref_is_mm a))
+//   [SMTPat (is_mm (grref_of a t rel))]
+// = ()
 
-let is_mm_grref_of
-  (#i: hh_rid)
-  (a: aref i)
-  (t: Type0)
-  (rel: preorder t)
-: Lemma
-  (requires (exists h . aref_live_at h a t rel))
-  (ensures ((exists h . aref_live_at h a t rel) /\ is_mm (grref_of a t rel) == aref_is_mm a))
-  [SMTPat (is_mm (grref_of a t rel))]
-= ()
+// let unused_in_gref_of
+//   (#i: rid)
+//   (a: aref i)
+//   (v: Type0)
+//   (rel: preorder v)
+//   (h: t)
+// : Lemma
+//   (requires (exists h . aref_live_at h a v rel))
+//   (ensures ((exists h . aref_live_at h a v rel) /\ (unused_in (grref_of a v rel) h <==> aref_unused_in a h)))
+//   [SMTPat (unused_in (grref_of a v rel) h)]
+// = ()
 
-let unused_in_gref_of
-  (#i: hh_rid)
-  (a: aref i)
-  (v: Type0)
-  (rel: preorder v)
-  (h: t)
-: Lemma
-  (requires (exists h . aref_live_at h a v rel))
-  (ensures ((exists h . aref_live_at h a v rel) /\ (unused_in (grref_of a v rel) h <==> aref_unused_in a h)))
-  [SMTPat (unused_in (grref_of a v rel) h)]
-= ()
+// let sel_rref_of
+//   (#i: rid)
+//   (a: aref i)
+//   (v: Type0)
+//   (rel: preorder v)
+//   (h1 h2: t)
+// : Lemma
+//   (requires (aref_live_at h1 a v rel /\ aref_live_at h2 a v rel))
+//   (ensures (aref_live_at h2 a v rel /\ sel h1 (rref_of h2 a v rel) == sel h1 (grref_of a v rel)))
+//   [SMTPat (sel h1 (rref_of h2 a v rel))]
+// = ()
 
-let sel_rref_of
-  (#i: hh_rid)
-  (a: aref i)
-  (v: Type0)
-  (rel: preorder v)
-  (h1 h2: t)
-: Lemma
-  (requires (aref_live_at h1 a v rel /\ aref_live_at h2 a v rel))
-  (ensures (aref_live_at h2 a v rel /\ sel h1 (rref_of h2 a v rel) == sel h1 (grref_of a v rel)))
-  [SMTPat (sel h1 (rref_of h2 a v rel))]
-= ()
+// let upd_rref_of
+//   (#i: rid)
+//   (a: aref i)
+//   (v: Type0)
+//   (rel: preorder v)
+//   (h1 h2: t)
+//   (x: v)
+// : Lemma
+//   (requires (aref_live_at h1 a v rel /\ aref_live_at h2 a v rel))
+//   (ensures (aref_live_at h2 a v rel /\ upd h1 (rref_of h2 a v rel) x == upd h1 (grref_of a v rel) x))
+//   [SMTPat (upd h1 (rref_of h2 a v rel) x)]
+// = ()
 
-let upd_rref_of
-  (#i: hh_rid)
-  (a: aref i)
-  (v: Type0)
-  (rel: preorder v)
-  (h1 h2: t)
-  (x: v)
-: Lemma
-  (requires (aref_live_at h1 a v rel /\ aref_live_at h2 a v rel))
-  (ensures (aref_live_at h2 a v rel /\ upd h1 (rref_of h2 a v rel) x == upd h1 (grref_of a v rel) x))
-  [SMTPat (upd h1 (rref_of h2 a v rel) x)]
-= ()
-
-abstract let extend (r:hh_rid) (n:int) (c:int)
-  :Pure hh_rid (requires True) (ensures (fun s -> s `extends` r /\ Cons? (reveal s) /\ Cons?.hd (reveal s) == (c, n) /\ hh_color s == c))
+abstract let extend (r:rid) (n:int) (c:int)
+  :Pure rid (requires True) (ensures (fun s -> s `extends` r /\ Cons? (reveal s) /\ Cons?.hd (reveal s) == (c, n) /\ color s == c))
   = elift1 (fun r -> (c, n)::r) r
 
-abstract let extend_monochrome (r:hh_rid) (n:int)
-  : Pure hh_rid (requires True) (ensures (fun s -> s `extends` r /\ Cons? (reveal s) /\ Cons?.hd (reveal s) == ((hh_color r), n) /\ hh_color s == hh_color r))
+abstract let extend_monochrome (r:rid) (n:int)
+  : Pure rid (requires True) (ensures (fun s -> s `extends` r /\ Cons? (reveal s) /\ Cons?.hd (reveal s) == ((color r), n) /\ color s == color r))
 = elift1 (fun r -> ((match r with | [] -> 0 | (c, _) :: _ -> c), n)::r) r
 
 
-abstract let alloc (#a:Type0) (rel:preorder a) (id:hh_rid) (init:a) (mm:bool) (m:t{m `Map.contains` id})
-  :Tot (p:(mrref id a rel * t){let (r, h) = Heap.alloc rel (Map.sel m id) init mm in
-                               (as_ref (fst p) == r /\
-                               snd p == Map.upd m id h)})
-  = let (r, h) = Heap.alloc rel (Map.sel m id) init mm in
-    r, Map.upd m id h
+// abstract let alloc (#a:Type0) (rel:preorder a) (id:rid) (init:a) (mm:bool) (m:t{m `Map.contains` id})
+//   :Tot (p:(mrref id a rel * t){let (r, h) = Heap.alloc rel (Map.sel m id) init mm in
+//                                (as_ref (fst p) == r /\
+//                                snd p == Map.upd m id h)})
+//   = let (r, h) = Heap.alloc rel (Map.sel m id) init mm in
+//     r, Map.upd m id h
