ulib/FStar.Monotonic.HyperStack.fst
@@ -3,18 +3,12 @@ module FStar.Monotonic.HyperStack
 open FStar.Preorder
 open FStar.Monotonic.HyperHeap
 module Map  = FStar.Map
-module HH   = FStar.Monotonic.HyperHeap
 
-type rid = HH.hh_rid
-let root = HH.hh_root
-let parent (r:rid{r =!= root}) :Tot rid = HH.parent r
-let color (x:rid) :GTot int = HH.hh_color x
-let extends (r1 r2:rid) = HH.extends r1 r2
-let disjoint (r1 r2:rid) = HH.disjoint r1 r2
-let includes (r1 r2:rid) = HH.includes r1 r2
-let disjoint_regions (s1 s2:Set.set rid) = HH.disjoint_regions s1 s2
+include FStar.Monotonic.HyperHeap
 
-let is_in (r:rid) (h:HH.t) = h `Map.contains` r
+type hmap = t
+
+let is_in (r:rid) (h:hmap) = h `Map.contains` r
 
 let is_stack_region r = color r > 0
 let is_eternal_color c = c <= 0
@@ -28,40 +22,40 @@ let is_below r1 r2      = r2 `is_above` r1
 let is_strictly_below r1 r2 = r1 `is_below` r2 && r1<>r2
 let is_strictly_above r1 r2 = r1 `is_above` r2 && r1<>r2
 
-abstract let downward_closed (h:HH.t) =
+abstract let downward_closed (h:hmap) =
   forall (r:rid). r `is_in` h  //for any region in the memory
         ==> (r=root    //either is the root
             \/ (forall (s:rid). r `is_above` s  //or, any region beneath it
                           /\ s `is_in` h   //that is also in the memory
                      ==> (is_stack_region r = is_stack_region s))) //must be of the same flavor as itself
 
-abstract let tip_top (tip:rid) (h:HH.t) =
+abstract let tip_top (tip:rid) (h:hmap) =
   forall (r:sid). r `is_in` h <==> r `is_above` tip  
 
-let is_tip (tip:rid) (h:HH.t) =
+let is_tip (tip:rid) (h:hmap) =
   (is_stack_region tip \/ tip=root)                                  //the tip is a stack region, or the root
   /\ tip `is_in` h                                                      //the tip is active
   /\ tip_top tip h                      //any other sid activation is a above (or equal to) the tip
 
 let rid_last_component (r:rid) :GTot int
   = let open FStar.List.Tot in
-    let r = HH.reveal r in
+    let r = reveal r in
     if length r = 0 then 0
     else snd (hd r)
 
 (*
  * AR: marking it abstract, else it has a high-chance of firing even with a pattern
  *)
-abstract let rid_ctr_pred (h:HH.t) (n:int) =
+abstract let rid_ctr_pred (h:hmap) (n:int) =
   forall (r:rid).{:pattern (h `Map.contains` r)}
                h `Map.contains` r ==> rid_last_component r < n
 
-let hh = h:HH.t{root `is_in` h /\ HH.map_invariant h /\ downward_closed h}        //the memory itself, always contains the root region, and the parent of any active region is active
+let hh = h:hmap{root `is_in` h /\ map_invariant h /\ downward_closed h}    //the memory itself, always contains the root region, and the parent of any active region is active
 
 noeq type mem =
   | HS : rid_ctr:int
        -> h:hh{rid_ctr_pred h rid_ctr}
-       -> tip:rid{tip `is_tip` h}                                                   //the id of the current top-most region
+       -> tip:rid{tip `is_tip` h}    //the id of the current top-most region
        -> mem
 
 (****** tip_top related lemmas ******)
@@ -137,7 +131,7 @@ let lemma_rid_ctr_pred ()
 //   = ()
 (*****)
 
-let empty_mem (m:HH.t) = 
+let empty_mem (m:hmap) = 
   let empty_map = Map.restrict (Set.empty) m in 
   let h = Map.upd empty_map root Heap.emp in
   let tip = root in
@@ -153,7 +147,7 @@ let test1 (m:mem) (r:rid{r `is_above` m.tip}) =
 let test2 (m:mem) (r:sid{m.tip `is_above` r /\ m.tip <> r}) =
    assert (~ (r `is_in` m.h))
 
-let dc_elim (h:HH.t{downward_closed h}) (r:rid{r `is_in` h /\ r <> root}) (s:rid)
+let dc_elim (h:hmap{downward_closed h}) (r:rid{r `is_in` h /\ r <> root}) (s:rid)
   : Lemma (r `is_above` s /\ s `is_in` h ==> is_stack_region r = is_stack_region s)
   = ()
 
@@ -165,7 +159,7 @@ let test4 (m:mem) (r:rid{r <> root /\ is_eternal_region r /\ r `is_above` m.tip 
   : Lemma (~ (r `is_in` m.h))
   = ()
 
-let eternal_region_does_not_overlap_with_tip (m:mem) (r:rid{is_eternal_region r /\ not (HH.disjoint r m.tip) /\ r<>root /\ is_stack_region m.tip})
+let eternal_region_does_not_overlap_with_tip (m:mem) (r:rid{is_eternal_region r /\ not (disjoint r m.tip) /\ r<>root /\ is_stack_region m.tip})
   : Lemma (requires True)
           (ensures (~ (r `is_in` m.h)))
   = root_has_color_zero()
@@ -176,7 +170,7 @@ let remove_elt (#a:eqtype) (s:Set.set a) (x:a) = Set.intersect s (Set.complement
 
 let popped m0 m1 =
   poppable m0
-  /\ HH.parent m0.tip = m1.tip
+  /\ parent m0.tip = m1.tip
   /\ Set.equal (Map.domain m1.h) (remove_elt (Map.domain m0.h) m0.tip)
   /\ Map.equal m1.h (Map.restrict (Map.domain m1.h) m0.h)
 
@@ -186,7 +180,7 @@ let pop (m0:mem{poppable m0}) : Tot mem =
   let h0 = m0.h in
   let h1 = Map.restrict dom m0.h in
   let tip0 = m0.tip in
-  let tip1 = HH.parent tip0 in
+  let tip1 = parent tip0 in
   assert (forall (r:sid). Map.contains h1 r ==>
   	    (forall (s:sid). includes s r ==> Map.contains h1 s));
   HS m0.rid_ctr h1 tip1
@@ -197,7 +191,7 @@ let pop (m0:mem{poppable m0}) : Tot mem =
 private
 noeq
 type mreference' (a:Type) (rel:preorder a) =
-  | MkRef : frame:rid -> mrref:HH.mrref frame a rel -> mreference' a rel
+  | MkRef : frame:rid -> ref:Heap.mref a rel -> mreference' a rel
 
 let mreference a rel = mreference' a rel
 
@@ -206,27 +200,28 @@ let frameOf (#a:Type) (#rel:preorder a) (r:mreference a rel)
   : Tot rid
   = r.frame
 
-let mrref_of (#a:Type) (#rel:preorder a) (r:mreference a rel)
-  : Tot (HH.mrref (frameOf r) a rel)
-  = r.mrref
-
-let mk_mreference (#id:rid) (#a:Type) (#rel:preorder a)
-                  (r:HH.mrref id a rel)
+let mk_mreference (#a:Type) (#rel:preorder a) (id:rid)
+                  (r:Heap.mref a rel)
   : Tot (mreference a rel)
   = MkRef id r
 
 //Hopefully we can get rid of this one
-let as_ref #a #rel (x:mreference a rel)
+abstract let as_ref #a #rel (x:mreference a rel)
   : Tot (Heap.mref a rel)
-  = HH.as_ref (mrref_of x)
+  = MkRef?.ref x
 
 //And make this one abstract
 let as_addr #a #rel (x:mreference a rel)
   : GTot nat
   = Heap.addr_of (as_ref x)
 
-let is_mm (#a:Type) (#rel:preorder a) (r:mreference a rel) : GTot bool =
-  HH.is_mm (mrref_of r)
+let lemma_as_ref_inj (#a:Type) (#rel:preorder a) (r:mreference a rel)
+  :Lemma (requires True) (ensures (mk_mreference (frameOf r) (as_ref r) == r))
+         [SMTPat (as_ref r)]
+  = ()
+
+let is_mm (#a:Type) (#rel:preorder a) (r:mreference a rel) :GTot bool =
+  Heap.is_mm (as_ref r)
 
 // Warning: all of the type aliases below get special support for KreMLin
 // extraction. If you rename or add to this list,
@@ -267,10 +262,13 @@ let contains (#a:Type) (#rel:preorder a) (m:mem) (s:mreference a rel) :GTot bool
   live_region m i && (FStar.StrongExcludedMiddle.strong_excluded_middle (Heap.contains (Map.sel m.h i) (as_ref s)))
 
 let unused_in (#a:Type) (#rel:preorder a) (r:mreference a rel) (h:mem) :GTot bool =
-  HH.unused_in (mrref_of r) h.h
+  let i = frameOf r in
+  not (Map.contains h.h i) ||
+  FStar.StrongExcludedMiddle.strong_excluded_middle (Heap.unused_in (as_ref r) (Map.sel h.h i))
 
 let contains_ref_in_its_region (#a:Type) (#rel:preorder a) (h:mem) (r:mreference a rel) :GTot bool =
-  HH.contains_ref_in_its_region (mrref_of r) h.h
+  let i = frameOf r in
+  FStar.StrongExcludedMiddle.strong_excluded_middle (Heap.contains (Map.sel h.h i) (as_ref r))
 
 let fresh_ref (#a:Type) (#rel:preorder a) (r:mreference a rel) (m0:mem) (m1:mem) :Type0 =
   let i = frameOf r in
@@ -282,43 +280,45 @@ let fresh_region (i:rid) (m0 m1:mem) =
 abstract private let stronger_fresh_region_was_redundant (i:rid) (m0 m1:mem)  //AR: because of map_invariant
   :Tot unit
   = let stronger_fresh_region (i:rid) (m0 m1:mem) =
-      (forall j. HH.includes i j ==> not (j `is_in` m0.h)) /\
+      (forall j. includes i j ==> not (j `is_in` m0.h)) /\
       i `is_in` m1.h
     in
     assert (fresh_region i m0 m1 ==> stronger_fresh_region i m0 m1)
 
 abstract val lemma_extends_fresh_disjoint: i:rid -> j:rid -> ipar:rid -> jpar:rid
-                               -> m0:mem{HH.map_invariant m0.h} -> m1:mem{HH.map_invariant m1.h} ->
+                               -> m0:mem{map_invariant m0.h} -> m1:mem{map_invariant m1.h} ->
   Lemma (requires (fresh_region i m0 m1
                   /\ fresh_region j m0 m1
                   /\ Map.contains m0.h ipar
                   /\ Map.contains m0.h jpar
-                  /\ HH.extends i ipar
-                  /\ HH.extends j jpar
+                  /\ extends i ipar
+                  /\ extends j jpar
                   /\ i<>j))
-        (ensures (HH.disjoint i j))
+        (ensures (disjoint i j))
         [SMTPat (fresh_region i m0 m1);
          SMTPat (fresh_region j m0 m1);
-         SMTPat (HH.extends i ipar);
-         SMTPat (HH.extends j jpar)]
+         SMTPat (extends i ipar);
+         SMTPat (extends j jpar)]
 let lemma_extends_fresh_disjoint i j ipar jpar m0 m1 = ()
-
 
 (*
  * AR: why is this not enforcing live_region ?
  *)
 let sel (#a:Type) (#rel:preorder a) (m:mem) (s:mreference a rel)
   : GTot a
-  = m.h.[mrref_of s]
+  = Heap.sel (Map.sel m.h (frameOf s)) (as_ref s)
 
 let upd (#a:Type) (#rel:preorder a) (m:mem) (s:mreference a rel{live_region m (frameOf s)}) (v:a)
   : GTot mem
-  = HS m.rid_ctr (m.h.[mrref_of s] <- v) m.tip
+  = let i = frameOf s in
+    HS m.rid_ctr (Map.upd m.h i (Heap.upd (Map.sel m.h i) (as_ref s) v)) m.tip
 
 let alloc (#a:Type0) (rel:preorder a) (id:rid) (init:a) (mm:bool) (m:mem{m.h `Map.contains` id})
-  :Tot (mreference a rel * mem)
-  = let (r, h) = HH.alloc rel id init mm m.h in
-    (mk_mreference r), (HS m.rid_ctr h m.tip)
+  :Tot (p:(mreference a rel * mem){let (r, h) = Heap.alloc rel (Map.sel m.h id) init mm in
+                                   as_ref (fst p) == r /\
+				   (snd p).h == Map.upd m.h id h})
+  = let r, h = Heap.alloc rel (Map.sel m.h id) init mm in
+    (mk_mreference id r), (HS m.rid_ctr (Map.upd m.h id h) m.tip)
 
 let free (#a:Type0) (#rel:preorder a) (r:mreference a rel{is_mm r}) (m:mem{m `contains` r})
   :Tot mem
@@ -340,19 +340,20 @@ let sel_tot (#a:Type) (#rel:preorder a) (m:mem) (r:mreference a rel{m `contains`
 
 let fresh_frame (m0:mem) (m1:mem) =
   not (Map.contains m0.h m1.tip) /\
-  HH.parent m1.tip = m0.tip      /\
+  parent m1.tip = m0.tip         /\
   m1.h == Map.upd m0.h m1.tip Heap.emp
 
 let hs_push_frame (m:mem) :Tot (m':mem{fresh_frame m m'})
-  = let new_tip_rid = HH.extend m.tip m.rid_ctr 1 in
-    HS (m.rid_ctr + 1) (Map.upd m.h new_tip_rid Heap.emp) new_tip_rid
+  = let new_tip_rid = extend m.tip m.rid_ctr 1 in
+    let h1 = Map.upd m.h new_tip_rid Heap.emp in
+    HS (m.rid_ctr + 1) h1 new_tip_rid
 
 let new_eternal_region (m:mem) (parent:rid{is_eternal_region parent /\ m.h `Map.contains` parent})
                        (c:option int{None? c \/ is_eternal_color (Some?.v c)})
   :Tot (t:(rid * mem){fresh_region (fst t) m (snd t)})
   = let new_rid =
-      if None? c then HH.extend_monochrome parent m.rid_ctr
-      else HH.extend parent m.rid_ctr (Some?.v c)
+      if None? c then extend_monochrome parent m.rid_ctr
+      else extend parent m.rid_ctr (Some?.v c)
     in
     let h1 = Map.upd m.h new_rid Heap.emp in
     new_rid, HS (m.rid_ctr + 1) h1 m.tip
@@ -360,32 +361,29 @@ let new_eternal_region (m:mem) (parent:rid{is_eternal_region parent /\ m.h `Map.
 let lemma_sel_same_addr (#a:Type0) (#rel:preorder a) (h:mem) (r1:mreference a rel) (r2:mreference a rel)
   :Lemma (requires (frameOf r1 == frameOf r2 /\ h `contains` r1 /\ as_addr r1 = as_addr r2 /\ is_mm r1 == is_mm r2))
          (ensures  (h `contains` r2 /\ sel h r1 == sel h r2))
-= let m = Map.sel h.h (frameOf r1) in
-  FStar.Monotonic.Heap.lemma_sel_same_addr m (as_ref r1) (as_ref r2)
+  = let m = Map.sel h.h (frameOf r1) in
+    FStar.Monotonic.Heap.lemma_sel_same_addr m (as_ref r1) (as_ref r2)
 
 let lemma_sel_same_addr' (#a:Type0) (#rel:preorder a) (h:mem) (r1:mreference a rel) (r2:mreference a rel)
   :Lemma (requires (frameOf r1 == frameOf r2 /\ h `contains` r1 /\ as_addr r1 = as_addr r2 /\ is_mm r1 == is_mm r2))
          (ensures  (h `contains` r2 /\ sel h r1 == sel h r2))
 	 [SMTPat (sel h r1); SMTPat (sel h r2)]
-= let m = Map.sel h.h (frameOf r1) in
-  FStar.Monotonic.Heap.lemma_sel_same_addr m (as_ref r1) (as_ref r2)
+  = lemma_sel_same_addr h r1 r2
 
 let lemma_upd_same_addr (#a:Type0) (#rel:preorder a) (h:mem) (r1 r2:mreference a rel) (x: a)
   :Lemma (requires (frameOf r1 == frameOf r2 /\ (h `contains` r1 \/ h `contains` r2) /\
                     as_addr r1 == as_addr r2 /\ is_mm r1 == is_mm r2))
          (ensures  (h `contains` r1 /\ h `contains` r2 /\ upd h r1 x == upd h r2 x))
-= if StrongExcludedMiddle.strong_excluded_middle (h `contains` r1) then
-    lemma_sel_same_addr h r1 r2
-  else lemma_sel_same_addr h r2 r1
+  = if StrongExcludedMiddle.strong_excluded_middle (h `contains` r1) then
+      lemma_sel_same_addr h r1 r2
+    else lemma_sel_same_addr h r2 r1
 
 let lemma_upd_same_addr' (#a:Type0) (#rel:preorder a) (h:mem) (r1 r2:mreference a rel) (x: a)
   :Lemma (requires (frameOf r1 == frameOf r2 /\ (h `contains` r1 \/ h `contains` r2) /\
                     as_addr r1 == as_addr r2 /\ is_mm r1 == is_mm r2))
          (ensures  (h `contains` r1 /\ h `contains` r2 /\ upd h r1 x == upd h r2 x))
          [SMTPat (upd h r1 x); SMTPat (upd h r2 x)]
-= if StrongExcludedMiddle.strong_excluded_middle (h `contains` r1) then
-    lemma_sel_same_addr h r1 r2
-  else lemma_sel_same_addr h r2 r1
+  = lemma_upd_same_addr h r1 r2 x
 
 let equal_domains (m0:mem) (m1:mem) =
   m0.tip = m1.tip /\
@@ -411,10 +409,10 @@ let lemma_equal_stack_domains_trans (m0:mem) (m1:mem) (m2:mem) : Lemma
   = ()
 
 let modifies (s:Set.set rid) (m0:mem) (m1:mem) =
-  HH.modifies_just s m0.h m1.h /\ m0.tip=m1.tip
+  modifies_just s m0.h m1.h /\ m0.tip=m1.tip
 
 let modifies_transitively (s:Set.set rid) (m0:mem) (m1:mem) =
-  HH.modifies s m0.h m1.h /\ m0.tip=m1.tip
+  FStar.Monotonic.HyperHeap.modifies s m0.h m1.h /\ m0.tip=m1.tip
 
 let heap_only (m0:mem) = m0.tip = root
 
@@ -431,9 +429,9 @@ private let lemma_pop_is_popped (m0:mem{poppable m0})
   = let m1 = pop m0 in
     assert (Set.equal (Map.domain m1.h) (remove_elt (Map.domain m0.h) m0.tip))
 
-let modifies_one id h0 h1 = HH.modifies_one id h0.h h1.h
+let modifies_one id h0 h1 = modifies_one id h0.h h1.h
 let modifies_ref (id:rid) (s:Set.set nat) (h0:mem) (h1:mem) =
-  HH.modifies_rref id s h0.h h1.h /\ h1.tip=h0.tip
+  Heap.modifies s (Map.sel h0.h id) (Map.sel h1.h id) /\ h1.tip=h0.tip
 
 let lemma_upd_1 #a #rel (h:mem) (x:mreference a rel) (v:a{rel (sel h x) v}) : Lemma
   (requires (contains h x))
@@ -465,11 +463,6 @@ let above_tip_is_live (#a:Type) (#rel:preorder a) (m:mem) (x:mreference a rel) :
   (ensures (frameOf x `is_in` m.h))
   = ()
 
-let coerce_mrref (#id1:rid) (#id2:rid) (#a:Type) (#rel:preorder a)
-                 (r:mrref id1 a rel{id1 == id2})
-    : mrref id2 a rel
-    = r
-
 noeq type some_ref =
   | Ref : #a:Type0 -> #rel:preorder a -> mreference a rel -> some_ref
 
@@ -496,7 +489,7 @@ let eternal_disjoint_from_tip (h:mem{is_stack_region h.tip})
                               (r:rid{is_eternal_region r /\
                                      r<>root /\
                                      r `is_in` h.h})
-   : Lemma (HH.disjoint h.tip r)
+   : Lemma (disjoint h.tip r)
    = ()
 
 ////////////////////////////////////////////////////////////////////////////////
@@ -562,17 +555,17 @@ let f (a:Type0) (b:Type0) (rel_a:preorder a) (rel_b:preorder b) (rel_n:preorder 
 noeq abstract type aref: Type0 =
 | ARef:
     (aref_region: rid) ->
-    (aref_aref: HH.aref aref_region) ->
+    (aref_aref: Heap.aref) ->
     aref
 
-abstract let dummy_aref : aref = ARef _ (HH.dummy_aref root)
+abstract let dummy_aref : aref = ARef root Heap.dummy_aref
 
 abstract let aref_equal
   (a1 a2: aref)
 : Ghost bool
   (requires True)
   (ensures (fun b -> b == true <==> a1 == a2))
-= a1.aref_region = a2.aref_region && HH.aref_equal a1.aref_aref a2.aref_aref
+= a1.aref_region = a2.aref_region && Heap.aref_equal a1.aref_aref a2.aref_aref
 
 (* Introduction rule *)
 
@@ -580,8 +573,8 @@ abstract let aref_of
   (#t: Type)
   (#rel: preorder t)
   (r: mreference t rel)
-: Tot aref
-= ARef (frameOf r) (HH.aref_of (mrref_of r))
+  : Tot aref
+  = ARef (frameOf r) (Heap.aref_of (as_ref r))
 
 (* Operators lifted from reference *)
 
@@ -602,7 +595,7 @@ abstract let frameOf_aref_of
 abstract let aref_as_addr
   (a: aref)
 : GTot nat
-= HH.addr_of_aref a.aref_aref
+= Heap.addr_of_aref a.aref_aref
 
 abstract let aref_as_addr_aref_of
   (#t: Type)
@@ -611,12 +604,12 @@ abstract let aref_as_addr_aref_of
 : Lemma
   (aref_as_addr (aref_of r) == as_addr r)
   [SMTPat (aref_as_addr (aref_of r))]
-= HH.addr_of_aref_of (mrref_of r)
+= Heap.addr_of_aref_of (as_ref r)
 
 abstract let aref_is_mm
   (r: aref)
 : GTot bool
-= HH.aref_is_mm r.aref_aref
+= Heap.aref_is_mm r.aref_aref
 
 abstract let is_mm_aref_of
   (#t: Type)
@@ -625,14 +618,14 @@ abstract let is_mm_aref_of
 : Lemma
   (aref_is_mm (aref_of r) == is_mm r)
   [SMTPat (aref_is_mm (aref_of r))]
-= HH.is_mm_aref_of (mrref_of r)
+= Heap.is_mm_aref_of (as_ref r)
 
 abstract let aref_unused_in
   (a: aref)
   (h: mem)
 : GTot Type0
 = ~ (live_region h a.aref_region) \/
-  HH.aref_unused_in a.aref_aref h.h
+  Heap.aref_unused_in a.aref_aref (Map.sel h.h a.aref_region)
 
 abstract let unused_in_aref_of
   (#t: Type)
@@ -642,7 +635,7 @@ abstract let unused_in_aref_of
 : Lemma
   (aref_unused_in (aref_of r) h <==> unused_in r h)
   [SMTPat (aref_unused_in (aref_of r) h)]
-= HH.unused_in_aref_of (mrref_of r) h.h
+= Heap.unused_in_aref_of (as_ref r) (Map.sel h.h (frameOf r))
 
 abstract
 val contains_aref_unused_in: #a:Type -> #rel: preorder a -> h:mem -> x:mreference a rel -> y:aref -> Lemma
@@ -652,7 +645,7 @@ val contains_aref_unused_in: #a:Type -> #rel: preorder a -> h:mem -> x:mreferenc
 let contains_aref_unused_in #a #rel h x y =
   if frameOf x = frameOf_aref y
   then 
-    Heap.contains_aref_unused_in (Map.sel h.h (frameOf x)) (as_ref x) (HH.as_heap_aref y.aref_aref) // HH.contains_ref_aref_unused_in h.h (mrref_of x) y.aref_aref
+    Heap.contains_aref_unused_in (Map.sel h.h (frameOf x)) (as_ref x) y.aref_aref
   else ()
 
 (* Elimination rule *)
@@ -665,7 +658,7 @@ let aref_live_at
   (rel: preorder v)
 : GTot Type0
 = live_region h a.aref_region
-  /\ HH.aref_live_at h.h a.aref_aref v rel
+  /\ Heap.aref_live_at (Map.sel h.h a.aref_region) a.aref_aref v rel
 
 abstract
 let greference_of
@@ -675,7 +668,7 @@ let greference_of
 : Ghost (mreference v rel)
   (requires (exists h . aref_live_at h a v rel))
   (ensures (fun _ -> True))
-= MkRef a.aref_region (HH.grref_of a.aref_aref v rel)
+= MkRef a.aref_region (Heap.gref_of a.aref_aref v rel)
 
 abstract
 let reference_of
@@ -686,7 +679,7 @@ let reference_of
 : Pure (mreference v rel)
   (requires (aref_live_at h a v rel))
   (ensures (fun x -> aref_live_at h a v rel /\ frameOf x == frameOf_aref a /\ as_addr x == aref_as_addr a /\ is_mm x == aref_is_mm a))
-= MkRef a.aref_region (HH.rref_of h.h a.aref_aref v rel)
+= MkRef a.aref_region (Heap.ref_of (Map.sel h.h a.aref_region) a.aref_aref v rel)
 
 abstract
 let aref_live_at_aref_of
@@ -746,7 +739,7 @@ let as_addr_greference_of
   (requires (exists h . aref_live_at h a t rel))
   (ensures ((exists h . aref_live_at h a t rel) /\ as_addr (greference_of a t rel) == aref_as_addr a))
   [SMTPat (as_addr (greference_of a t rel))]
-= assert (addr_of (grref_of a.aref_aref t rel) == addr_of_aref a.aref_aref)
+= ()
 
 abstract
 let is_mm_greference_of
